Update the definition of EvalM for the run mechanism Implement the mechanism to transform an ArrowP spec to a cf spec Fix a few bugs

translator/monadic/cfMonadLib.sml
@@ -1,0 +1,76 @@
+structure cfMonadLib (* :> cfMonadLib *) = struct
+
+open cfAppTheory cfTacticsLib ml_monad_translatorTheory cfMonadTheory
+
+val PURE_tm = ``PURE : ('a -> v -> bool) -> ('a, 'b) H``;
+fun mk_app_of_ArrowP_goal spec = let
+    val spec = PURE_REWRITE_RULE[ArrowM_def] spec
+    val arrow_RI = concl spec |> rator |> rator
+    val f_const = concl spec |> rator |> rand
+    val fv_const = concl spec |> rand
+    val H = arrow_RI |> rator |> rator |> rand
+    val state_type = type_of H |> dest_type |> snd |> List.hd
+    val state_var = mk_var("state", state_type)
+    val p_var = mk_var("p", ``:unit ffi_proj``)
+
+    (* Create variables for the HOL and CakeML parameters, retrieve the refinement invariants *)
+    fun get_params arrow_RI n = let
+	val (comb_tm, params) = strip_comb arrow_RI
+	val ri = rator arrow_RI |> rand |> rand
+	val arrow_RI' = rand arrow_RI
+	val comb_tm = rator arrow_RI'
+	val x = mk_var("x"^(Int.toString n), type_of ri |> dest_type |> snd |> List.hd)
+	val xv = mk_var("xv"^(Int.toString n), ``:v``)
+	val x_triple = (x, xv, ri)
+    in if same_const PURE_tm comb_tm then let
+	   val arrow_RI' = rand arrow_RI'
+	   val (params_v, ret_invs) = get_params arrow_RI' (n+1)
+       in (x_triple::params_v, ret_invs) end
+       else ([x_triple], (rator arrow_RI' |> rand, rand arrow_RI'))
+    end
+    val (params_info, (ret_inv, exn_inv)) = get_params arrow_RI 1
+    val ri_hyps = List.map (fn (x, xv, ri) => list_mk_comb(ri, [x, xv])) params_info
+    val params = List.map #1 params_info
+
+    (* Start the recursion *)
+    val current_f = list_mk_comb (f_const, List.take(params, List.length params - 1))
+    val (last_x, last_xv, last_ri) = List.last params_info
+    val xl = List.map #1 params_info
+    val xvl = List.map #2 params_info
+    val params_info = List.tl(List.rev params_info)
+    val fv_var = mk_var("fv", ``:v``)
+    val gv_var = mk_var("gv", ``:v``)
+
+    val th = ISPECL[last_ri, ret_inv, exn_inv, current_f, gv_var, H, last_x, last_xv, state_var] ArrowP_MONAD_to_app |> SPEC_ALL |> UNDISCH
+
+    val Q = concl th |> rand |> rand
+    val Q_abs = mk_abs(state_var, Q)
+
+    (* Perform the recursion *)
+    (* val (x, xv, ri) = List.hd params_info *)
+    fun mk_app_rec th ((x, xv, ri)::x_info) = let
+	val A = ri
+	val B = concl th |> dest_imp |> fst |> rator |> rator
+	val (xv2, xvl) = concl th |> dest_imp |> snd |> rator |> rator |> rand |> dest_comb
+	val xv2 = rand xv2
+	val f_tm = concl th |> dest_imp |> fst |> rator |> rand |> rator
+	
+	val assum = GENL[state_var, gv_var] th
+	val imp_th = ISPECL[A, B, f_tm, fv_var, x, xv, xv2, xvl, H, Q_abs] ArrowP_PURE_to_app
+			|> SPEC_ALL |> UNDISCH |> BETA_RULE
+	val th = MP imp_th assum |> SPEC_ALL |> Thm.INST [fv_var |-> gv_var]
+    in mk_app_rec th x_info end
+      | mk_app_rec th [] = th
+    val th = mk_app_rec th params_info
+
+    (* Instantiate the CakeML function variable and remove the ArrowP hypothesis *)
+    val th = MP (Thm.INST[gv_var |-> fv_const] th) spec
+
+    (* Undischarge the refinement invariants for the arguments *)
+    val th = List.foldr (fn (a, th) => DISCH a th) th ri_hyps
+
+    (* Generalize the variables *)
+    val th = GENL[state_var, p_var] th |> GENL xvl |> GENL xl
+in th end
+
+end
