translator/monadic/examples/arrayStateProgScript.sml
@@ -64,7 +64,6 @@ val arrays_init_list = List.map (fn ((x1, x2, x3, x4, x5, x6, x7), x) => (x1, x,
 
 val store_hprop_name = "STATE_STORE";
 val state_type = ``:state_refs``;
-val EXN_RI = ``STATE_EXN_TYPE``;
 val exn_ri_def = STATE_EXN_TYPE_def;
 
 (* Initialize the store *)
