translator/monadic/examples/runProgScript.sml
@@ -1,0 +1,615 @@
+open ml_monadBaseLib ml_monadBaseTheory
+open ml_monad_translatorTheory ml_monadStoreLib ml_monad_translatorLib
+
+val _ = new_theory "arrayStateProg"
+val _ = ParseExtras.temp_loose_equality();
+val _ = patternMatchesLib.ENABLE_PMATCH_CASES();
+val _ = monadsyntax.temp_add_monadsyntax()
+
+val _ = temp_overload_on ("monad_bind", ``st_ex_bind``);
+val _ = temp_overload_on ("monad_unitbind", ``\x y. st_ex_bind x (\z. y)``);
+val _ = temp_overload_on ("monad_ignore_bind", ``\x y. st_ex_bind x (\z. y)``);
+val _ = temp_overload_on ("return", ``st_ex_return``);
+
+val _ = hide "state";
+
+val _ = (use_full_type_names := false);
+
+(* Register the types used for the translation *)
+val _ = register_type ``:'a # 'b``;
+val _ = register_type ``:'a list``;
+val _ = register_type ``:'a option``;
+val _ = register_type ``:('a, 'b) exc``;
+val _ = register_type ``:unit``;
+
+(* Create the data type to handle the references *)
+val _ = Hol_datatype `
+  state_refs = <| the_num : num ;
+	          the_num_array : num list ;
+                  the_int_array : int list |>`;
+
+(* Data type for the exceptions *)
+val _ = Hol_datatype`
+  state_exn = Fail of string | ReadError of unit | WriteError of unit`;
+
+val _ = register_exn_type ``:state_exn``;
+val STATE_EXN_TYPE_def = theorem"STATE_EXN_TYPE_def";
+
+val _ = register_type ``:state_refs``;
+val STATE_REFS_TYPE_def = theorem"STATE_REFS_TYPE_def";
+
+(* Monadic functions to handle the exceptions *)
+val exceptions_funs = define_monad_exception_functions ``:state_exn`` ``:state_refs``;
+val _ = temp_overload_on ("failwith", ``raise_Fail``);
+
+(* Define the functions used to access the elements of the state_refs data_type *)
+val access_funs = define_monad_access_funs (``:state_refs``);
+val [(the_num_name, get_the_num_def, set_the_num_def),
+     (the_num_array_name, get_the_num_array_def, set_the_num_array_def),
+     (the_int_array_name, get_the_int_array_def, set_the_int_array_def)] = access_funs;
+
+val sub_exn = ``ReadError ()``;
+val update_exn = ``WriteError ()``;
+val array_access_funs = (List.tl access_funs);
+val array_manip_funs = define_Marray_manip_funs array_access_funs sub_exn update_exn;
+
+(* Prepare the translation *)
+val init_num_def = Define `init_num = (0 : num)`;
+val refs_init_list = [(the_num_name, init_num_def, get_the_num_def, set_the_num_def)];
+
+val init_num_array_def = Define `init_num_array = [] : num list`;
+val init_int_array_def = Define `init_int_array = [] : int list`;
+val arrays_init_values = [init_num_array_def, init_int_array_def];
+val arrays_init_list = List.map (fn ((x1, x2, x3, x4, x5, x6, x7), x) => (x1, x, x2, x3, x4, x5, x6, x7)) (zip array_manip_funs arrays_init_values);
+
+val infer_init_state = ``<|the_num := 0; the_num_array := []; the_int_array := []|>``;
+
+val store_hprop_name = "STATE_STORE";
+val state_type = ``:state_refs``;
+val EXN_RI = ``STATE_EXN_TYPE``;
+val exn_ri_def = STATE_EXN_TYPE_def;
+
+val refs_manip_list = List.map (fn (x, _, y, z) => (x, y, z)) refs_init_list;
+val arrays_manip_list = List.map (fn (x1, _, x2, x3, x4, x5, x6, x7) => (x1, x2, x3, x4, x5, x6, x7)) arrays_init_list;
+
+val translation_parameters = translate_dynamic_init_fixed_store refs_manip_list arrays_manip_list store_hprop_name state_type exn_ri_def;
+
+(* Initialize the store *)
+(* val (translation_parameters, store_trans_result) = translate_static_init_fixed_store refs_init_list arrays_init_list store_hprop_name state_type STATE_EXN_TYPE_def; *)
+
+(* Initialize the translation *)
+(* val store_pred_exists = SOME(#store_pred_exists_thm store_trans_result); *)
+val store_pred_exists = NONE : thm option;
+val _ = init_translation translation_parameters store_pred_exists exc_ri_def [];
+
+(* Prove the theorems necessary to handle the exceptions *)
+val (raise_functions, handle_functions) = unzip exceptions_funs;
+val exn_thms = add_raise_handle_functions raise_functions handle_functions STATE_EXN_TYPE_def
+
+(* Monadic translations *)
+val test2_def = Define `test2 n = the_num_array_sub n`;
+val def = test2_def |> m_translate;
+
+val test3_def = Define `test3 n x = update_the_num_array n x`;
+val def = test2_def |> m_translate;
+
+val test4_def = Define `test4 n x = alloc_the_num_array n x`;
+val def = test3_def |> m_translate;
+
+val test5_def = Define `
+test5 n z =
+    do
+	alloc_the_num_array n z;
+        return ()
+    od`;
+val def = test5_def |> m_translate;
+val test5_trans_th = m_translate test5_def;
+
+val test6_def = Define `
+test6 n z = test5 n z`;
+val def = test6_def;
+val test6_trans_th = m_translate test6_def;
+
+val test7_def = Define `
+(test7 [] = return 0) /\ ((test7 (x::l)) = (do x <- test7 l; return (x+1) od))`;
+val def = test7_def;
+val test7_v_th = m_translate test7_def;
+
+val test8_def = Define `
+test8 l = test7 l`;
+val test8_v_th = m_translate test8_def;
+
+val test9_def = Define `
+test9 n m z =
+   do
+       test5 n z;
+       x <- test2 m;
+       return x
+   od`;
+val test9_v_th = m_translate test9_def;
+
+(* New definitions for ml_monadBaseTheory *)
+val _ = ParseExtras.temp_tight_equality();
+
+fun evaluate_unique_result_tac (g as (asl, w)) = let
+    val asl = List.map ASSUME asl
+    val uniques = mapfilter (MATCH_MP evaluate_unique_result) asl
+in simp uniques g end;
+
+(* Test *)
+set_trace "assumptions" 1
+
+val current_state = get_state(get_ml_prog_state());
+val current_env = get_env(get_ml_prog_state());
+
+val spec = test9_v_th
+val original_spec = spec;
+
+val spec_info_pat = ``nsLookup (merge_env (LOCAL_ENV : v sem_env) env).v (Short NAME) = SOME EXPR``;
+
+
+val initial_state = mk_var("s", ``:unit semanticPrimitives$state``);
+
+val (name, def) = List.hd ref_name_def_pairs;
+
+val evaluate_let_opref = Q.store_thm("evaluate_let_opref",
+`Eval env exp1 P ==>
+?junk v. evaluate F env s (Let (SOME vname) (App Opref [exp1]) exp2) = evaluate F (write vname (Loc (LENGTH (s.refs ++ junk))) env) (s with refs := s.refs ++ junk ++ [Refv v]) exp2 /\ P v`,
+rw[Eval_def]
+\\ first_x_assum(qspec_then `s.refs` STRIP_ASSUME_TAC)
+\\ IMP_RES_TAC evaluate_empty_state_IMP
+\\ qexists_tac `refs'`
+\\ qexists_tac `res`
+\\ simp[]
+\\ irule EQ_EXT
+\\ rw[Once evaluate_cases]
+\\ rw[Once evaluate_cases]
+\\ rw[Once evaluate_cases]
+\\ evaluate_unique_result_tac
+\\ rw[Once evaluate_cases]
+\\ rw[do_app_def, store_alloc_def]
+\\ fs[write_def, namespaceTheory.nsOptBind_def]
+\\ rw[Once DISJ_COMM]
+\\ rw[Once evaluate_cases]
+\\ rw[Once evaluate_cases]
+\\ evaluate_unique_result_tac
+\\ rw[Once evaluate_cases]
+\\ rw[do_app_def, store_alloc_def]
+\\ rw[Once evaluate_cases]
+\\ evaluate_unique_result_tac
+\\ rw[Once evaluate_cases]
+\\ rw[Once evaluate_cases]
+\\ evaluate_unique_result_tac
+\\ rw[Once evaluate_cases]
+\\ rw[with_same_ffi]);
+
+val EvalSt_Let_Fun = Q.store_thm("EvalSt_Let_Fun",
+`EvalSt (merge_env (write vname (Closure (merge_env env1 env0) xv fexp) env1) env0) exp P refs H ==>
+EvalSt (merge_env env1 env0) (Let (SOME vname) (Fun xv fexp) exp) P refs H`,
+rw[EvalSt_def]
+\\ last_x_assum IMP_RES_TAC
+\\ first_x_assum(qspec_then `junk` STRIP_ASSUME_TAC)
+\\ rw[Once evaluate_cases]
+\\ rw[Once evaluate_cases]
+\\ rw[namespaceTheory.nsOptBind_def]
+\\ fs[write_def, merge_env_def]
+\\ metis_tac[]);
+
+val merge_env_bind_empty = Q.store_thm("merge_env_bind_empty",
+`merge_env <| v := Bind [] []; c := Bind [] [] |> env  = env`,
+rw[merge_env_def]
+\\ Cases_on `env`
+\\ Cases_on `n`
+\\ Cases_on `n0`
+\\ rw[namespaceTheory.nsAppend_def, sem_env_component_equality]);
+
+val EvalSt_Opref = Q.store_thm("EvalSt_Opref",
+`Eval (merge_env <|v := Bind binds []; c := Bind [] []|> env0) state_exp (STATE_TYPE state) ==>
+Eval (merge_env <| v := Bind binds []; c := Bind [] [] |> env0) get_ref_expr ((STATE_TYPE --> TYPE) (\state. get_val state)) ==>
+(!loc. EvalSt (merge_env <| v := Bind ((loc_name, loc)::binds) []; c := Bind [] [] |> env0) exp P state (\state. REF_REL TYPE loc (get_val state) * H state)) ==>
+EvalSt (merge_env <| v := Bind binds []; c := Bind [] [] |> env0)
+(Let (SOME loc_name) (App Opref [App Opapp [get_ref_expr; state_exp]]) exp) P state (\state. H state)`,
+rw[EvalSt_def]
+\\ rw[Once evaluate_cases]
+\\ rw[Once evaluate_cases]
+\\ rw[Once evaluate_cases]
+\\ fs[Eval_def]
+\\ last_x_assum(qspec_then `s.refs ++ junk` STRIP_ASSUME_TAC)
+\\ first_x_assum(fn x => MATCH_MP evaluate_empty_state_IMP_junk x |> ASSUME_TAC)
+\\ evaluate_unique_result_tac
+\\ rw[Once evaluate_cases]
+\\ last_x_assum(qspec_then `s.refs ++ junk ++ refs'` STRIP_ASSUME_TAC)
+\\ FULL_SIMP_TAC pure_ss [GSYM APPEND_ASSOC]
+\\ `s.refs ++ (junk ++ (refs' ++ refs'')) = s.refs ++ (junk ++ refs') ++ refs''` by simp[]
+\\ pop_assum(fn x => FULL_SIMP_TAC pure_ss [x])
+\\ first_x_assum(fn x => MATCH_MP evaluate_empty_state_IMP_junk x |> ASSUME_TAC)
+\\ rw[Once evaluate_cases]
+\\ evaluate_unique_result_tac
+\\ rw[Once evaluate_cases]
+\\ fs[Arrow_def]
+\\ first_x_assum(qspec_then `state` ASSUME_TAC)
+\\ fs[AppReturns_def]
+\\ first_x_assum(qspec_then `res` IMP_RES_TAC)
+\\ first_x_assum(qspec_then `s.refs ++ junk ++ refs' ++ refs''` STRIP_ASSUME_TAC)
+\\ rw[]
+\\ FULL_SIMP_TAC pure_ss [GSYM APPEND_ASSOC]
+\\ `s.refs ++ (junk ++ (refs' ++ (refs'' ++ refs'''))) = s.refs ++ (junk ++ (refs' ++ refs'')) ++ refs'''` by simp[]
+\\ pop_assum(fn x => FULL_SIMP_TAC pure_ss [x])
+\\ first_x_assum(fn x => MATCH_MP evaluate_empty_state_IMP_junk x |> ASSUME_TAC)
+\\ fs[]
+\\ evaluate_unique_result_tac
+\\ rw[Once evaluate_cases]
+\\ evaluate_unique_result_tac
+\\ rw[Once evaluate_cases]
+\\ rw[do_app_def, store_alloc_def]
+\\ rw[namespaceTheory.nsOptBind_def]
+\\ rw[with_same_ffi]
+\\ qpat_abbrev_tac `loc = LENGTH junk + L`
+\\ last_x_assum(qspecl_then [`Loc loc`, `s with refs := s.refs ++ junk ++ refs' ++ refs'' ++ refs''' ++ [Refv u]`, `p`] ASSUME_TAC)
+\\ first_assum(fn x => let val a = concl x |> dest_imp |> fst in sg `^a` end)
+>-(
+    rw[REFS_PRED_def]
+    \\ rw[GSYM STAR_ASSOC]
+    \\ rw[Once STAR_def]
+    \\ qexists_tac `store2heap_aux (LENGTH (s.refs ++ junk ++ refs' ++ refs'' ++ refs''')) [Refv u]`
+    \\ qexists_tac `st2heap p (s with refs := s.refs ++ junk ++ refs' ++ refs'' ++ refs''')`
+    \\ PURE_REWRITE_TAC[Once SPLIT_SYM]
+    \\ rw[STATE_SPLIT_REFS]
+    >-(
+	rw[REF_REL_def]
+	\\ rw[SEP_CLAUSES, SEP_EXISTS_THM]
+	\\ qexists_tac `u`
+        \\ EXTRACT_PURE_FACTS_TAC
+	\\ rw[REF_HPROP_SAT_EQ, cfStoreTheory.store2heap_aux_def])
+    \\ rw[Once (GSYM GC_STAR_GC), STAR_ASSOC]
+    \\ rw[Once STAR_def]
+    \\ qexists_tac `st2heap p (s with refs := s.refs)`
+    \\ qexists_tac `store2heap_aux (LENGTH s.refs) (junk ++ refs' ++ refs'' ++ refs''')`
+    \\ PURE_REWRITE_TAC[GSYM APPEND_ASSOC]
+    \\ rw[STATE_SPLIT_REFS, SAT_GC]
+    \\ fs[REFS_PRED_def, with_same_refs])
+\\ qpat_x_assum `A ==> R` IMP_RES_TAC
+\\ first_x_assum(qspec_then `[]` STRIP_ASSUME_TAC)
+\\ fs[merge_env_def]
+\\ Cases_on `env0`
+\\ Cases_on `n`
+\\ Cases_on `n0`
+\\ fs[namespaceTheory.nsBind_def, namespaceTheory.nsAppend_def]
+\\ evaluate_unique_result_tac
+\\ qexists_tac `refs2`
+\\ fs[REFS_PRED_FRAME_def]
+\\ rw[]
+\\ first_x_assum(qspec_then `F' * GC` ASSUME_TAC)
+\\ first_assum(fn x => let val a = concl x |> dest_imp |> fst in sg `^a` end)
+>-(
+    rw[GSYM STAR_ASSOC]
+    \\ rw[Once STAR_def]
+    \\ qexists_tac `store2heap_aux (LENGTH (s.refs ++ junk ++ refs' ++ refs'' ++ refs''')) [Refv u]`
+    \\ qexists_tac `st2heap p (s with refs := s.refs ++ junk ++ refs' ++ refs'' ++ refs''')`
+    \\ PURE_REWRITE_TAC[Once SPLIT_SYM]
+    \\ rw[STATE_SPLIT_REFS]
+    >-(
+	rw[REF_REL_def]
+	\\ rw[SEP_CLAUSES, SEP_EXISTS_THM]
+	\\ qexists_tac `u`
+        \\ EXTRACT_PURE_FACTS_TAC
+	\\ rw[REF_HPROP_SAT_EQ, cfStoreTheory.store2heap_aux_def])
+    \\ rw[STAR_ASSOC]
+    \\ rw[Once STAR_def]
+    \\ qexists_tac `st2heap p (s with refs := s.refs)`
+    \\ qexists_tac `store2heap_aux (LENGTH s.refs) (junk ++ refs' ++ refs'' ++ refs''')`
+    \\ PURE_REWRITE_TAC[GSYM APPEND_ASSOC]
+    \\ rw[STATE_SPLIT_REFS, SAT_GC]
+    \\ fs[REFS_PRED_def, with_same_refs])
+\\ qpat_x_assum `A ==> R` IMP_RES_TAC
+\\ fs[GSYM STAR_ASSOC, GC_STAR_GC]
+\\ first_x_assum(fn x => PURE_ONCE_REWRITE_RULE[STAR_COMM] x |> ASSUME_TAC)
+\\ fs[STAR_ASSOC]
+\\ first_x_assum(fn x => MATCH_MP GC_ABSORB_R x |> ASSUME_TAC)
+\\ fs[]);
+
+val Eval_lookup_var = Q.store_thm("Eval_lookup_var",
+`!env vname xv x TYPE. nsLookup env.v (Short vname) = SOME xv ==>
+(Eval env (Var (Short vname)) (TYPE x) <=> TYPE x xv)`,
+rw[Eval_def]
+\\ EQ_TAC
+>-(simp[Once evaluate_cases] \\ rw[] \\ metis_tac[])
+\\ rw[Once evaluate_cases]
+\\ rw[state_component_equality]);
+
+val STATE_REFS_TYPE_def = theorem"STATE_REFS_TYPE_def";
+
+val test_10_def = Define `test10 n m z refs = insert_monad (test9 n m z) refs`;
+
+val Long_tm = ``namespace$Long : tvarN -> (tvarN, tvarN) id -> (tvarN, tvarN) id ``;
+fun get_exn_constructs () = let
+    val exn_type_def = !EXN_TYPE_def_ref
+    val exn_type_conjs = CONJUNCTS exn_type_def
+    val deep_cons_list = List.map (fn x => concl x |> strip_forall |> snd |> rhs |> strip_exists
+				|> snd |> dest_conj |> fst |> rhs |> rator) exn_type_conjs
+    val deep_names = List.map (fn x => rand x |> rand |> dest_pair |> fst) deep_cons_list
+
+    (* Get the module name *)
+    val deep_type = List.hd deep_cons_list |> rand |> rand |> dest_pair |> snd |> rand
+    val uses_module_name = strip_comb deep_type |> fst |> same_const Long_tm
+    val module_name = if uses_module_name then SOME(strip_comb deep_type |> snd |> List.hd)
+		      else NONE
+in (deep_names, module_name) end;
+
+fun create_local_defs th = let
+    (* Retrieve the lookup assumptions for the functions definitions *)
+    val LOCAL_ENV = mk_var("LOCAL_ENV", ``:v sem_env``)
+    val NAME = mk_var("NAME", ``:tvarN``)
+    val EXPR = mk_var("EXPR", ``:v``)
+    val pat = ``nsLookup ^LOCAL_ENV.v (Short ^NAME) = SOME ^EXPR``
+    val substs =  mapfilter (match_term pat) (hyp th)
+    val lookup_info = List.map (fn (tms, _) => (Term.subst tms NAME, Term.subst tms EXPR)) substs
+    val lookup_info = List.filter(fn (x, y) => not(is_var y)) lookup_info
+
+    fun get_env_var expr = rator expr |> rator |> rand |> rator |> rand
+    fun compute_env_index env = let
+	val env_name = dest_var env |> fst
+	val env_index_str = String.extract(env_name, String.size local_environment_var_name, NONE)
+	val index = string_to_int env_index_str
+    in index end
+
+    (* Sort the lookup assumptions *)
+    val lookup_info = List.map (fn (name, expr) => let val env = get_env_var expr in
+				(compute_env_index env, env, name, expr) end) lookup_info
+    fun assum_order (i1 : int, _, _, _) (i2 : int, _, _, _) = i1 > i2
+    val lookup_info = Lib.sort assum_order lookup_info
+    val lookup_info = List.map (fn (_, x, y, z) => (x, y, z)) lookup_info
+
+    (* Create the function definitions (Let expressions) *)
+    val current_env = concl th |> rator |> rator |> rator |> rator |> rand |> rator |> rand
+    val all_envs = List.map (fn (x, _, _) => x) lookup_info
+    val last_env = List.last all_envs
+    val all_envs = current_env::(List.take(all_envs, List.length all_envs - 1))
+    val lookup_info = zip all_envs lookup_info
+
+    fun create_fun_let ((env_var2, (env_var1, name, fexp)), th) = let
+	(* Build the new environment *)
+	val env0 = rator fexp |> rator |> rand |> rand
+	val env1 = env_var1
+	val vname = name
+	val xv = rator fexp |> rand
+	val fexp = rand fexp
+
+	val nenv = ``(write ^vname (Closure (merge_env ^env1 ^env0) ^xv ^fexp) ^env1)``
+
+	(* Replace the environment and create the Let expression *)
+	val th' = Thm.INST [env_var2 |-> nenv] th
+	val th' = MATCH_MP EvalSt_Let_Fun th'
+
+	(* Remove the appropriate nsLookup assumption *)
+	val assum = ``nsLookup (merge_env ^nenv ^env0).v (Short ^vname) =
+		     SOME (Closure (merge_env (^env_var1) ^env0) ^xv ^fexp)``
+	val assum_rw = EVAL assum
+	val th' = DISCH assum th' |> SIMP_RULE bool_ss [assum_rw]
+    in th' end
+
+    val th = List.foldl create_fun_let th lookup_info
+in th end;
+
+fun translate_insert_monad def = let
+    (* Decompose the definition *)
+    val (def_lhs, def_rhs) = concl test_10_def |> strip_forall |> snd |> dest_eq
+    val Mvar = mk_var("M", ``:('a, 'b, 'c) M``)
+    val Svar = mk_var("S", ``:'a``)
+    val (tms, tys) = match_term ``insert_monad ^Mvar ^Svar`` def_rhs
+    val monad_tm = Term.subst tms (Term.inst tys Mvar)
+    val state_tm = Term.subst tms (Term.inst tys Svar)
+    val (monad_f, monad_params) = strip_comb monad_tm
+
+    (* Construct the Eval predicates for the parameters *)
+    fun var_create_Eval tm = let
+	val (name,ty) = dest_var tm
+	val inv = get_type_inv ty
+	val str = stringSyntax.fromMLstring name
+	val result = ASSUME (mk_comb(``Eval env (Var (Short ^str))``,mk_comb(inv,tm)))
+	val result = MATCH_MP (ISPEC_EvalM Eval_IMP_PURE) result
+    in check_inv "var" tm result end
+    val params_evals = List.map var_create_Eval monad_params
+
+    (* Get the monadic specification *)
+    val monad_th = lookup_dynamic_v_thm monad_f
+    val monad_th = (MATCH_MP Eval_IMP_PURE monad_th)
+		 |> ISPEC (!H)
+		 |> PURE_REWRITE_RULE[GSYM ArrowM_def]
+    
+    (* Insert the parameters *)
+    val monad_th = List.foldl (fn (x, th) => MATCH_MP(MATCH_MP EvalM_ArrowM th) x)
+			      monad_th params_evals
+
+    (* Translate the insert_monad construct *)
+    val env = concl monad_th |> rator |> rator |> rator |> rand
+    val x = concl monad_th |> rator |> rand |> rand
+    val exp = concl monad_th |> rator |> rator |> rand
+    val MONAD_TYPE = concl monad_th |> rator |> rand |> rator
+    val EXN_TYPE = rand MONAD_TYPE
+    val TYPE = rator MONAD_TYPE |> rand
+    val vname = stringSyntax.fromMLstring "vname"
+    val (exn_cons_names, exn_module_name) = get_exn_constructs ()
+    val cons_names = mk_list(exn_cons_names, ``:tvarN``)
+    val th = case exn_module_name of
+		 SOME module_name =>
+		 ISPECL [cons_names, module_name, vname, TYPE, EXN_TYPE, x, exp,
+			 !H, state_tm, env] EvalM_insert_monad_MODULE
+	       | NONE =>
+		 ISPECL [cons_names, vname, TYPE, EXN_TYPE, x, exp,
+			 !H, state_tm, env] EvalM_insert_monad_SIMPLE
+    (* Prove the assumptions *)
+    val [EXN_assum, distinct_assum, vname_assum1, vname_assum2] = List.take(
+	    concl th |> strip_imp |> fst, 4)
+    val EXN_th = prove(EXN_assum, rw[] \\ Cases_on `e` \\ fs[!EXN_TYPE_def_ref])
+    val th = MP th EXN_th
+		
+    val distinct_rw = SIMP_CONV list_ss [] distinct_assum
+    val vname_rw1 = SIMP_CONV list_ss [] vname_assum1
+    val vname_rw2 = SIMP_CONV list_ss [] vname_assum2
+    val th = SIMP_RULE bool_ss [EXN_rw, distinct_rw, vname_rw1, vname_rw2] th
+    val th = MP th monad_th
+
+    (* Undischarge the lookup assumptions *)
+    val every_lookup_assum = concl th |> dest_imp |> fst
+    val every_lookup_rw = SIMP_CONV list_ss [] every_lookup_assum
+    val th = SIMP_RULE bool_ss [every_lookup_rw, GSYM AND_IMP_INTRO] th |> UNDISCH_ALL
+
+    (* Replace the environment *)
+    val nenv = get_current_env()
+    val th = Thm.INST [env |-> nenv] th
+
+    (* Create the local function definitions *)
+    val th = create_local_defs th
+
+    (* Remove the last environment *)
+    val empty_env = ``<| v := Bind [] []; c := Bind [] [] |> : v sem_env``
+    val th = Thm.INST [last_env |-> empty_env] th |> PURE_REWRITE_RULE [merge_env_bind_empty]
+
+    (*
+     * Instantiate the environment 0
+     *)
+    val global_env = get_env(get_curr_prog_state())
+    val params_bindings = List.map(fn x => (concl x |> rator |> rator |> rand |> rand |> rand,
+					    concl x |> rator |> rand |> rand)) params_evals
+    val state_var = concl th |> rator |> rand
+    val state_var_eval = hol2deep state_var
+    val state_var_binding = ((concl state_var_eval |> rator |> rand |> rand |> rand), state_var)
+    
+    (* Create variables for the deep embeddings of the parameters *)
+    val fvl = HOLset.listItems(FVL ((concl th)::(hyp th)) empty_varset)
+    val deep_params = List.map (fn (n, var) => variant fvl (mk_var((dest_var var |> fst) ^ "_v", ``:v``))) params_bindings
+    val hol_deep_pairs = List.map (fn ((n, x), xv) => (x, xv)) (zip params_bindings deep_params)
+    val deep_params_map = List.foldr (fn ((x, xv), m) => Redblackmap.insert(m, x, xv)) (Redblackmap.mkDict Term.compare) hol_deep_pairs
+
+    val params_bindings_v = List.map (fn ((n, x), xv) => (n, xv)) (zip params_bindings deep_params)
+    val params_bindings_v = List.map mk_pair params_bindings_v
+    val params_bindings_v = mk_list(params_bindings_v, ``:tvarN # v``)
+
+    (* val params_invs_hyps = List.map (fn ((n, x), xv) => list_mk_comb(get_type_inv (type_of x), [x, xv])) (zip params_bindings deep_params) *)
+
+    (* Create the environment 0 and substitute it *)
+    val env0 = ``merge_env <| v := Bind ^params_bindings_v []; c := Bind [] [] |> ^global_env``
+    val th = Thm.INST [local_environment_var_0 |-> env0] th
+    
+    (* Simplify the assumptions *)
+    val assums = hyp th
+    val lookup_cons_assums = List.filter (can (match_term ``lookup_cons vname env = SOME t``)) assums
+    val lookup_cons_rws = mapfilter(fn x => EVAL x |> EQT_ELIM) lookup_cons_assums
+    val th = List.foldr (fn (a, th) => MP (DISCH (concl a) th) a) th lookup_cons_rws
+    val assums = hyp th
+    val nsLookup_assums = List.filter (can (match_term ``nsLookup env id = SOME var``)) assums
+    val nsLookup_assums_rws = mapfilter(fn x => EVAL x |> EQT_ELIM) nsLookup_assums
+    val th = List.foldr (fn (a, th) => MP (DISCH (concl a) th) a) th nsLookup_assums_rws
+    val assums = hyp th
+    val Eval_var_assums = List.filter (can (match_term ``Eval env exp (P x)``)) assums
+
+    fun rewrite_Eval_var (assum, th) = let
+	val env = rator assum |> rator |> rand
+	val vname = rator assum |> rand |> rand |> rand
+	val x = rand assum |> rand
+	val xv = Redblackmap.find (deep_params_map, x)
+	val TYPE = rand assum |> rator
+
+	val rw_th = ISPECL[env, vname, xv, x, TYPE] Eval_lookup_var
+	val rw_th_assum = concl rw_th |> dest_imp |> fst
+	val rw_th = MP rw_th (EVAL rw_th_assum |> EQT_ELIM)
+
+	val inv_to_eval = EQ_IMP_RULE rw_th |> snd |> UNDISCH
+	val th = MP (DISCH (concl inv_to_eval) th) inv_to_eval
+    in th end
+
+    val th = List.foldl rewrite_Eval_var th Eval_var_assums
+
+			(* Create the store *)
+
+
+
+Eval_def
+
+DB.apropos ``(x <=> T) <=> x``
+
+EVAL ``lookup_cons "Success" (merge_env auto_env_9 init_env)``
+``lookup_cons``
+
+val assum1 = List.nth(assums, 1)
+EVAL assum1
+
+    val assums = DISCH_ALL th' 
+    val clean_assumptions (DISCH_ALL th')
+
+lookup_cons_def
+
+EVAL ``NUM x y``
+    val all_param_bindings = List.map mk_pair all_param_bindings
+    val all_params_bindings = mk_list(all_param_bindings, ``:tvarN # v``)
+    val env0 = ``merge_env
+
+    val th' = Thm.INST[local_environment_var_0  |-> global_env] th |> DISCH_ALL
+
+
+    (* Create the store *)
+    fun create_local_store th = let
+	val th = PURE_REWRITE_RULE [!H_def, GSYM STAR_ASSOC] th
+	val state_var = concl th |> rator |> rand
+
+th
+EvalSt_Opref
+
+assums
+List.hd assums
+
+fun create_local_store refs_init_list arrays_init_list store_hprop_name =
+  let
+      val _ = if List.null refs_init_list andalso List.null arrays_init_list
+	      then raise (ERR "create_store" "need a non empty list of reference init values")
+	      else ()
+
+      val initial_state = mk_var("s", ``:unit semanticPrimitives$state``)
+      val initial_store = ``^initial_state.refs``
+      val initial_env = get_env(get_ml_prog_state())
+
+      (* Allocate the references *)
+      fun create_ref ((name, def), (s, env)) =
+	let
+	    val trans_th = abs_translate def
+	    val expr = rator (concl trans_th) |> rand
+	    val e = ``(App Opref [^expr])``
+	    (derive_eval_thm name e)
+
+
+	    val value_expr = 
+	    val init_name = concl def |> dest_eq |> fst |> dest_const |> fst
+	    val init_name = stringLib.fromMLstring init_name
+	    val e = ``(App Opref [Var (Short ^init_name)])``
+	    val _ = ml_prog_update (add_Dlet (derive_eval_thm name e) name [])
+	    val ref_def = DB.fetch (current_theory()) (name ^ "_def")
+	in
+	    (value_def, ref_def)
+	end
+      val ref_name_def_pairs = List.map (fn (n, d, _, _) => (n, d)) refs_init_list
+      val refs_trans_results = List.map create_ref ref_name_def_pairs
+
+      (* Allocate the arrays *)
+      fun create_array (name, def) =
+	let
+	    val init_name = concl def |> lhs |> dest_const |> fst
+
+	    val (array_v_def, array_loc_def, ref_def, eval_th) =
+		derive_eval_thm_ALLOCATE_EMPTY_ARRAY init_name def
+	    val _ = ml_prog_update(add_Dlet eval_th name [])
+         in
+	     (array_v_def, array_loc_def, ref_def)
+	end
+      val array_name_def_pairs = List.map (fn (n, d, _, _, _, _, _, _) => (n, d)) arrays_init_list
+      val arrays_trans_results = List.map create_array array_name_def_pairs
+  in
+    (initial_store, refs_trans_results, arrays_trans_results)
+  end;
+
+hol2deep ``state_refs x_3 x_2 x_1:state_refs``
+
+
+Net.listItems (!dynamic_specs)
+
+val _ = export_theory ();
